theories/imp_heap_bij.v
@@ -8,76 +8,398 @@ Require Import refframe.prepost.
 Require Import refframe.proof_techniques.
 Require Import refframe.imp.
 
+
+Implicit Types (p : prov).
+
 (** * imp_heap_bij *)
+Inductive heap_bij_elem :=
+| HBShared (p : prov) | HBOwned (p : player).
+Global Instance heap_bij_elem_eq_dec : EqDecision heap_bij_elem.
+Proof. solve_decision. Qed.
+Global Instance heap_bij_elem_inhabited : Inhabited heap_bij_elem := populate (HBOwned Prog).
+
+(* Naming scheme: pi for provenances in the implementation (right side
+of hb_bij), ps for provanences in the spec (left side) *)
+
 Record heap_bij := HeapBij {
-  hb_bij : gset (prov * prov);
-  hb_env : gset prov;
-  hb_prog : gset prov;
-  hb_disj_env : hb_env ## set_map snd hb_bij;
-  hb_disj_prog : hb_prog ## set_map snd hb_bij;
-  hb_disj_priv : hb_prog ## hb_env;
-  hb_iff p1 p2 p1' p2' : (p1, p2) ∈ hb_bij → (p1', p2') ∈ hb_bij → p1 = p1' ↔ p2 = p2'
+  hb_bij : gmap prov heap_bij_elem;
+  hb_players_i : gmap prov player;
+  hb_disj ps pi:
+   hb_bij !! ps = Some (HBShared pi) →
+   hb_players_i !! pi = None;
+  hb_iff pi ps ps' :
+   hb_bij !! ps = Some (HBShared pi) →
+   hb_bij !! ps' = Some (HBShared pi) →
+   ps = ps'
 }.
+Add Printing Constructor heap_bij.
+
+Ltac simplify_bij :=
+  repeat (simplify_eq; match goal with
+         | H1 : hb_bij ?bij !! ?ps1 = Some (HBShared ?pi),
+             H2 : hb_bij ?bij !! ?ps2 = Some (HBShared ?pi) |- _ =>
+             pose proof (hb_iff bij pi ps1 ps2 H1 H2); clear H2
+         end); simplify_eq.
+
+Lemma heap_bij_eq bij1 bij2 :
+  bij1 = bij2 ↔ hb_bij bij1 = hb_bij bij2 ∧ hb_players_i bij1 = hb_players_i bij2.
+Proof.
+  split; [naive_solver|]. move => [??]. destruct bij1, bij2 => /=. simplify_eq/=. f_equal.
+  (* TODO: get rid of this *)
+  all: apply proof_irrelevance.
+Qed.
 
 Global Program Instance imp_heap_bij_empty : Empty heap_bij :=
-  HeapBij ∅ ∅ ∅ _ _ _ _.
+  HeapBij ∅ ∅ _ _.
 Solve Obligations with set_solver.
 
-Definition hb_provs_right (bij : heap_bij) : gset prov :=
-  (set_map snd (hb_bij bij) ∪ hb_env bij ∪ hb_prog bij).
+(** hb_shared_i *)
+Definition hb_shared_i (bij : heap_bij) : gset prov :=
+  list_to_set (omap (λ x, if x.2 is HBShared p then Some p else None) (map_to_list (hb_bij bij))).
+Global Typeclasses Opaque hb_shared_i.
 
-Definition heap_bij_extend (p : player) (bij bij' : heap_bij) :=
-  hb_bij bij ⊆ hb_bij bij' ∧
-  (if p is Env then hb_env bij ⊆ hb_env bij' else hb_env bij = hb_env bij') ∧
-  (if p is Prog then hb_prog bij ⊆ hb_prog bij' else hb_prog bij = hb_prog bij').
+Lemma elem_of_hb_shared_i bij pi:
+  pi ∈ hb_shared_i bij ↔ ∃ ps, hb_bij bij !! ps = Some (HBShared pi).
+Proof.
+  rewrite /hb_shared_i elem_of_list_to_set elem_of_list_omap.
+  setoid_rewrite elem_of_map_to_list'.
+  split.
+  - move => [[??] /= [??]]. case_match; simplify_eq/=. naive_solver.
+  - move => [??]. by eexists (_, _).
+Qed.
 
-Global Instance heap_bij_extend_preorder p : PreOrder (heap_bij_extend p).
+(** hb_shared *)
+Definition hb_shared (bij : heap_bij) : gmap prov prov :=
+  (omap (λ v, if v is HBShared p then Some p else None) (hb_bij bij)).
+
+Lemma hb_shared_lookup bij ps :
+  hb_shared bij !! ps = hb_bij bij !! ps ≫= λ v, if v is HBShared p then Some p else None.
+Proof. apply lookup_omap. Qed.
+
+Lemma hb_shared_lookup_Some bij ps pi :
+  hb_shared bij !! ps = Some pi ↔ hb_bij bij !! ps = Some (HBShared pi).
+Proof. rewrite hb_shared_lookup. destruct (hb_bij bij !! ps) => //=. case_match; naive_solver. Qed.
+
+Lemma hb_shared_lookup_None bij ps :
+  hb_shared bij !! ps = None ↔ ∀ pi, hb_bij bij !! ps = Some (HBShared pi) → False.
+Proof. rewrite hb_shared_lookup. destruct (hb_bij bij !! ps) => //=. case_match; naive_solver. Qed.
+
+(** hb_shared_s *)
+Definition hb_shared_s (bij : heap_bij) : gset prov :=
+  (locked (dom _) (hb_shared bij)).
+
+Lemma elem_of_hb_shared_s bij ps :
+  ps ∈ hb_shared_s bij ↔ ∃ pi, hb_bij bij !! ps = Some (HBShared pi).
+Proof. rewrite /hb_shared_s; unlock. rewrite elem_of_dom /is_Some. f_equiv => ?. apply hb_shared_lookup_Some. Qed.
+
+(** hb_player_s *)
+Definition hb_player_s (pl : player) (bij : heap_bij) : gset prov :=
+  (locked (dom _) (filter (λ '(k, e), e = HBOwned pl) (hb_bij bij))).
+
+Lemma elem_of_hb_player_s pl bij ps :
+  ps ∈ hb_player_s pl bij ↔ hb_bij bij !! ps = Some (HBOwned pl).
+Proof.
+  unfold hb_player_s. unlock. rewrite elem_of_dom /is_Some. setoid_rewrite map_filter_lookup_Some.
+  naive_solver.
+Qed.
+
+Lemma not_elem_of_hb_player_s pl bij ps :
+  ps ∉ hb_player_s pl bij ↔ hb_bij bij !! ps ≠ Some (HBOwned pl).
+Proof. by rewrite elem_of_hb_player_s. Qed.
+
+Lemma hb_player_s_empty pl bij :
+  hb_player_s pl bij = ∅ ↔ (∀ ps, hb_bij bij !! ps ≠ Some (HBOwned pl)).
+Proof. rewrite set_eq. setoid_rewrite elem_of_hb_player_s. set_solver. Qed.
+
+(** hb_player_i *)
+Definition hb_player_i (pl : player) (bij : heap_bij) : gset prov :=
+  (locked (dom _) (filter (λ '(k, e), e = pl) (hb_players_i bij))).
+
+Lemma elem_of_hb_player_i pl bij pi :
+  pi ∈ hb_player_i pl bij ↔ hb_players_i bij !! pi = Some pl.
+Proof.
+  unfold hb_player_i. unlock. rewrite elem_of_dom /is_Some. setoid_rewrite map_filter_lookup_Some.
+  naive_solver.
+Qed.
+
+Lemma not_elem_of_hb_player_i pl bij pi :
+  pi ∉ hb_player_i pl bij ↔ hb_players_i bij !! pi ≠ Some pl.
+Proof. by rewrite elem_of_hb_player_i. Qed.
+
+Lemma hb_player_i_empty pl bij :
+  hb_player_i pl bij = ∅ ↔ (∀ ps, hb_players_i bij !! ps ≠ Some pl).
+Proof. rewrite set_eq. setoid_rewrite elem_of_hb_player_i. set_solver. Qed.
+
+(** hb_provs_i *)
+(* hb_provs_s is directly written as [dom _ (hb_bij bij)] *)
+
+Definition hb_provs_i (bij : heap_bij) : gset prov :=
+  dom _ (hb_players_i bij) ∪ hb_shared_i bij.
+
+Lemma elem_of_hb_provs_i bij pi :
+  pi ∈ hb_provs_i bij ↔ (∃ pl, hb_players_i bij !! pi = Some pl) ∨ ∃ ps, hb_bij bij !! ps = Some (HBShared pi).
+Proof. unfold hb_provs_i. rewrite elem_of_union elem_of_dom elem_of_hb_shared_i. naive_solver. Qed.
+
+(** general hb_bij *)
+Lemma heap_bij_eq_parts bij1 bij2 :
+  bij1 = bij2 ↔
+    hb_shared bij1 = hb_shared bij2 ∧
+    ∀ pl, hb_player_s pl bij1 = hb_player_s pl bij2 ∧ hb_player_i pl bij1 = hb_player_i pl bij2.
+Proof.
+  split; [naive_solver|]. move => [Hshared Hp]. apply heap_bij_eq.
+  split.
+  - apply map_eq => ?. apply option_eq => -[?|?]; rewrite -?hb_shared_lookup_Some -?elem_of_hb_player_s.
+    + naive_solver congruence.
+    + set_solver.
+  - apply map_eq => ?. apply option_eq => ?. rewrite -?elem_of_hb_player_i. set_solver.
+Qed.
+
+Global Instance heap_bij_subseteq : SubsetEq heap_bij :=
+  λ bij bij', ∀ ps pi, hb_bij bij !! ps = Some (HBShared pi) → hb_bij bij' !! ps = Some (HBShared pi).
+
+Global Instance heap_bij_preorder : PreOrder (⊆@{heap_bij}).
+Proof. unfold subseteq,heap_bij_subseteq. constructor; naive_solver. Qed.
+
+Definition heap_bij_extend (pl : player) (bij bij' : heap_bij) :=
+  bij ⊆ bij'
+  ∧ hb_player_s (opponent pl) bij = hb_player_s (opponent pl) bij'
+  ∧ hb_player_i (opponent pl) bij = hb_player_i (opponent pl) bij'.
+
+Global Instance heap_bij_extend_preorder pl : PreOrder (heap_bij_extend pl).
 Proof.
   unfold heap_bij_extend. constructor.
-  - move => *. destruct p;set_solver.
-  - move => *. destruct p;set_solver.
+  - move => *. done.
+  - move => *. destruct_all?. split; [by etrans|split; by etrans].
 Qed.
 Global Typeclasses Opaque heap_bij_extend.
 
-Program Definition heap_bij_add_loc (p1 p2 : prov) (bij : heap_bij)
-        (H : p1 ∉ set_map (D:=gset _) fst (hb_bij bij)) (_ : p2 ∉ hb_provs_right bij) :=
-  HeapBij ({[ (p1, p2 )]} ∪ hb_bij bij) (hb_env bij) (hb_prog bij) _ _ _ _.
+Local Ltac bij_solver := unfold heap_bij_extend, subseteq, heap_bij_subseteq in *; set_unfold; naive_solver.
+
+Program Definition heap_bij_add_shared (pi ps : prov) (bij : heap_bij)
+        (H : pi ∉ hb_provs_i bij) :=
+  HeapBij (<[ps := HBShared pi]> (hb_bij bij)) (hb_players_i bij) _ _.
 Next Obligation.
-  move => ?????. rewrite set_map_union_L. apply disjoint_union_r. split; [|apply hb_disj_env].
-  rewrite set_map_singleton_L disjoint_singleton_r. set_solver.
+  move => ??? Hnotin ??. move: Hnotin. rewrite elem_of_hb_provs_i => ?.
+  rewrite !lookup_insert_Some => ?. destruct_all?; simplify_eq/= => //; try naive_solver.
+  - apply eq_None_ne_Some => ??. naive_solver.
+  - by apply: hb_disj.
 Qed.
 Next Obligation.
-  move => ?????. rewrite set_map_union_L. apply disjoint_union_r. split; [|apply hb_disj_prog].
-  rewrite set_map_singleton_L disjoint_singleton_r. set_solver.
-Qed.
-Next Obligation. move => *. apply hb_disj_priv. Qed.
-Next Obligation.
-  move => ??? Hl Hr??????. set_unfold.
-  destruct_all?; simplify_eq => //.
-  - split => ?;  [contradict Hl | contradict Hr; left; left]; eexists (_,_); naive_solver.
-  - split => ?;  [contradict Hl | contradict Hr; left; left]; eexists (_,_); naive_solver.
-  - by apply: hb_iff.
+  move => ??? Hnotin ???. move: Hnotin. rewrite elem_of_hb_provs_i => ?.
+  rewrite !lookup_insert_Some => ??. destruct_all?; simplify_eq/= => //; try naive_solver.
+  by apply: hb_iff.
 Qed.
 
-Program Definition heap_bij_add_prog (p2 : prov) (bij : heap_bij) (_ : p2 ∉ hb_provs_right bij) :=
-  HeapBij (hb_bij bij) (hb_env bij) ({[ p2 ]} ∪ hb_prog bij) _ _ _ _.
-Next Obligation. move => ???. apply: hb_disj_env. Qed.
+Program Definition heap_bij_add_player (ps : prov) (pl : player) (bij : heap_bij) :=
+  HeapBij (<[ps := HBOwned pl]> (hb_bij bij)) (hb_players_i bij) _ _.
 Next Obligation.
-  move => ???. apply disjoint_union_l. split; [|apply hb_disj_prog].
-  rewrite disjoint_singleton_l. set_solver.
+  move => ?????.
+  rewrite !lookup_insert_Some => ?. destruct_all?; simplify_eq/= => //. by apply: hb_disj.
 Qed.
 Next Obligation.
-  move => ???. apply disjoint_union_l. split; [|apply hb_disj_priv].
-  rewrite disjoint_singleton_l. set_solver.
+  move => ??????.
+  rewrite !lookup_insert_Some => ??. destruct_all?; simplify_eq/= => //. by apply: hb_iff.
 Qed.
-Next Obligation. move => ????. apply: hb_iff. Qed.
+
+Program Definition heap_bij_delete (ps : prov) (bij : heap_bij) :=
+  HeapBij (delete ps (hb_bij bij)) (hb_players_i bij) _ _.
+Next Obligation.
+  move => ????.
+  rewrite !lookup_delete_Some => ?. destruct_all?; simplify_eq/= => //. by apply: hb_disj.
+Qed.
+Next Obligation.
+  move => ?????.
+  rewrite !lookup_delete_Some => ??. destruct_all?; simplify_eq/= => //. by apply: hb_iff.
+Qed.
+
+(* Definition heap_bij_map_player_bij (f : prov → player → player) (bij : heap_bij) : gmap prov heap_bij_elem := *)
+(*   map_imap (λ ps e, Some $ if e is HBOwned p then HBOwned (f ps p) else e) (hb_bij bij). *)
+
+(* Lemma heap_bij_map_player_bij_lookup f bij p2 : *)
+(*   heap_bij_map_player_bij f bij !! p2 = *)
+(*     (λ x, if x is HBOwned p then HBOwned (f p2 p) else x) <$> hb_bij bij !! p2. *)
+(* Proof. rewrite map_lookup_imap. by destruct (hb_bij bij !! p2). Qed. *)
+
+(* Lemma heap_bij_map_player_bij_lookup_shared f bij p2 p1: *)
+(*   heap_bij_map_player_bij f bij !! p2 = Some (HBShared p1) ↔ hb_bij bij !! p2 = Some (HBShared p1). *)
+(* Proof. *)
+(*   rewrite heap_bij_map_player_bij_lookup. rewrite fmap_Some. split; [|naive_solver]. *)
+(*   move => [[?|?][??]]//. naive_solver. *)
+(* Qed. *)
+
+(* Program Definition heap_bij_map_player (f : prov → player → player) (bij : heap_bij) := *)
+(*   HeapBij (heap_bij_map_player_bij f bij) _. *)
+(* Next Obligation. *)
+(*   move => ?????? /heap_bij_map_player_bij_lookup_shared?/heap_bij_map_player_bij_lookup_shared?. apply: hb_iff; naive_solver. *)
+(* Qed. *)
+
+(* Lemma heap_bij_map_player_subseteq_l f bij1 bij2: *)
+(*   heap_bij_map_player f bij1 ⊆ bij2 ↔ bij1 ⊆ bij2. *)
+(* Proof. unfold subseteq, heap_bij_subseteq. by setoid_rewrite heap_bij_map_player_bij_lookup_shared. Qed. *)
+
+(* Lemma heap_bij_map_player_subseteq_r f bij1 bij2: *)
+(*   bij1 ⊆ heap_bij_map_player f bij2 ↔ bij1 ⊆ bij2. *)
+(* Proof. unfold subseteq, heap_bij_subseteq. by setoid_rewrite heap_bij_map_player_bij_lookup_shared. Qed. *)
+
+(* (* Lemma elem_of_hb_player_s_map p x f bij : *) *)
+(* (*   x ∈ hb_player_s p (heap_bij_map_player f bij) ↔ f  *) *)
+
+(* only provenances which are shared in both bijections become shared
+in the merged bijection, otherwise they become private. *)
+Program Definition heap_bij_merge (bija bijb : heap_bij) :=
+  HeapBij ((λ x, if x is HBShared pi then default (HBOwned Prog) (hb_bij bija !! pi) else x) <$> hb_bij bijb)
+          (hb_players_i bija ∪ gset_to_gmap Prog (filter (λ pii,
+              map_Forall (λ pi pii', ¬ (pii' = pii ∧ pi ∈ hb_shared_i bijb))
+                         (hb_shared bija)) (hb_shared_i bija)))
+          _ _.
+Next Obligation.
+  move => ????. rewrite !lookup_fmap=> /fmap_Some[?[??]].
+  unfold default in *; repeat case_match; simplify_eq/=.
+  apply lookup_union_None. split; [by apply: hb_disj|].
+  rewrite lookup_gset_to_gmap_None. rewrite elem_of_filter.
+  move => [Hall _]. apply: Hall; [by rewrite hb_shared_lookup_Some|]. rewrite elem_of_hb_shared_i.
+  naive_solver.
+Qed.
+Next Obligation.
+  move => ?????. rewrite !lookup_fmap => /fmap_Some[?[??]] /fmap_Some[?[??]].
+  unfold default in *; repeat case_match; simplify_bij; simplify_eq/=; by simplify_bij.
+Qed.
+
+Lemma heap_bij_merge_lookup bijb bija ps :
+  hb_bij (heap_bij_merge bija bijb) !! ps =
+  (λ x, if x is HBShared pi then default (HBOwned Prog) (hb_bij bija !! pi) else x) <$> hb_bij bijb !! ps.
+Proof. by rewrite lookup_fmap. Qed.
+
+Lemma heap_bij_merge_player_i pii bijb bija pl:
+  pii ∈ hb_player_i pl (heap_bij_merge bija bijb) ↔
+    hb_players_i bija !! pii = Some pl ∨
+    ∃ pi, pl = Prog ∧ hb_bij bija !! pi = Some (HBShared pii) ∧ pi ∉ hb_shared_i bijb.
+Proof.
+  rewrite elem_of_hb_player_i /= lookup_union_Some_raw lookup_gset_to_gmap_Some elem_of_filter.
+  split => ?; destruct_all?; simplify_eq; try naive_solver.
+  - right. revert select (_ ∈ _). rewrite elem_of_hb_shared_i => -[??]. eexists _.
+    split; [done|]. split; [done|].
+    move => ?. revert select (map_Forall _ _). apply; [|done]. by rewrite hb_shared_lookup_Some.
+  - right. split_and!. { by apply: hb_disj. } { done. }
+    + move => ??. rewrite hb_shared_lookup_Some => ? [??]. simplify_bij. naive_solver.
+    + rewrite elem_of_hb_shared_i. naive_solver.
+Qed.
+Opaque heap_bij_merge.
+
+Lemma heap_bij_merge_player_s ps bijb bija pl:
+  ps ∈ hb_player_s pl (heap_bij_merge bija bijb) ↔
+    hb_bij bijb !! ps = Some (HBOwned pl) ∨ ∃ pi, hb_bij bijb !! ps = Some (HBShared pi) ∧
+       default (HBOwned Prog) (hb_bij bija !! pi) = HBOwned pl.
+Proof.
+  rewrite elem_of_hb_player_s heap_bij_merge_lookup fmap_Some.
+  destruct (hb_bij bijb !! ps) as [[]|]; naive_solver.
+Qed.
+
+Lemma heap_bij_merge_shared bijb bija ps pii :
+  hb_bij (heap_bij_merge bija bijb) !! ps = Some (HBShared pii) ↔
+     ∃ pi, hb_bij bijb !! ps = Some (HBShared pi) ∧ hb_bij bija !! pi = Some (HBShared pii).
+Proof.
+  simpl. rewrite heap_bij_merge_lookup fmap_Some.  split.
+  - move => [[p'|?][??]] //. destruct (hb_bij bija !! p') eqn:?; naive_solver.
+  - move => [?[Hl1 Hl2]]. eexists _. split; [done|] => /=. by rewrite Hl2.
+Qed.
+
+Lemma heap_bij_merge_shared_i bija bijb pii:
+  pii ∈ hb_shared_i (heap_bij_merge bija bijb) ↔
+    ∃ pi, hb_bij bija !! pi = Some (HBShared pii) ∧ pi ∈ hb_shared_i bijb.
+Proof.
+  rewrite !elem_of_hb_shared_i.
+  setoid_rewrite heap_bij_merge_shared.
+  setoid_rewrite elem_of_hb_shared_i.
+  naive_solver.
+Qed.
+
+Lemma heap_bij_merge_dom bijb bija :
+  dom (gset _) (hb_bij (heap_bij_merge bija bijb)) = dom _ (hb_bij bijb).
+Proof. apply set_eq => ?. by rewrite !elem_of_dom heap_bij_merge_lookup fmap_is_Some. Qed.
+
+Lemma heap_bij_merge_provs_i bija bijb pii:
+  pii ∈ hb_provs_i (heap_bij_merge bija bijb) ↔ pii ∈ hb_provs_i bija.
+Proof.
+  rewrite !elem_of_hb_provs_i.
+  setoid_rewrite heap_bij_merge_shared.
+  setoid_rewrite <-elem_of_hb_player_i at 1.
+  setoid_rewrite heap_bij_merge_player_i.
+  split; [naive_solver|]. move => [?|[pi Hpi]]. 1: naive_solver.
+  destruct (decide (pi ∈ hb_shared_i bijb)) as [Hps|Hps]; [|naive_solver].
+  rewrite elem_of_hb_shared_i in Hps. naive_solver.
+Qed.
+
+Lemma heap_bij_merge_prog_eq_s bija bijb bij' ps:
+  hb_player_s Prog (heap_bij_merge bija bijb) = hb_player_s Prog bij' →
+  hb_bij bij' !! ps = Some (HBOwned Prog) ↔
+  hb_bij bijb !! ps = Some (HBOwned Prog) ∨ (∃ pi,
+    hb_bij bijb !! ps = Some (HBShared pi) ∧ (∀ y, hb_bij bija !! pi = Some y → y = HBOwned Prog))
+  .
+Proof.
+  move => /set_eq/(_ ps). rewrite heap_bij_merge_player_s elem_of_hb_player_s.
+  setoid_rewrite default_eq_Some'. naive_solver.
+Qed.
+
+Lemma heap_bij_merge_prog_eq_i bija bijb bij' pii:
+  hb_player_i Prog (heap_bij_merge bija bijb) = hb_player_i Prog bij' →
+  hb_players_i bij' !! pii = Some Prog ↔
+  hb_players_i bija !! pii = Some Prog ∨ (∃ pi, hb_bij bija !! pi = Some (HBShared pii) ∧ pi ∉ hb_shared_i bijb)
+  .
+Proof. move => /set_eq/(_ pii). rewrite heap_bij_merge_player_i elem_of_hb_player_i. naive_solver. Qed.
+
+(* TODO: clean up the following lemmas *)
+Lemma heap_bij_merge_extend_env bija bijb bij' ps x:
+  heap_bij_extend Env (heap_bij_merge bija bijb) bij' →
+  hb_bij bij' !! ps = Some (HBOwned Env) →
+  hb_player_s Env bija = ∅ →
+  hb_bij bijb !! ps = Some x →
+  x = HBOwned Env.
+Proof.
+  move => [/=Hsub [Hprog ?]] Hbij' /hb_player_s_empty Hbija Hbijb.
+  destruct x as [pi|[]] => //=. 2: { move: Hprog => /heap_bij_merge_prog_eq_s. naive_solver. }
+  move: Hprog => /heap_bij_merge_prog_eq_s?.
+  destruct (hb_bij bija !! pi) as [[pii|[]]|] eqn:?; [|naive_solver..].
+  have := Hsub ps pii. rewrite heap_bij_merge_shared. naive_solver.
+Qed.
+
+Lemma heap_bij_merge_extend_a ps pi pii bija bijb bij' :
+  heap_bij_extend Env (heap_bij_merge bija bijb) bij' →
+  hb_bij bij' !! ps = Some (HBShared pii) →
+  hb_bij bijb !! ps = Some (HBShared pi) →
+  hb_player_s Env bija = ∅ →
+  hb_bij bija !! pi = Some (HBShared pii).
+Proof.
+  move => [/=Hsub [Hprog ?]] Hbij' Hbijb /hb_player_s_empty Hempty.
+  move: Hprog => /heap_bij_merge_prog_eq_s?.
+  destruct (hb_bij bija !! pi) as [[pii'|[]]|] eqn:Hbij1; simplify_eq; [|naive_solver..].
+  have := Hsub ps pii'. rewrite heap_bij_merge_shared. naive_solver.
+Qed.
+
+Lemma heap_bij_merge_extend_env_i bija bijb bij' pi pii:
+  heap_bij_extend Env (heap_bij_merge bija bijb) bij' →
+  hb_bij bija !! pi = Some (HBShared pii) →
+  hb_players_i bij' !! pii ≠ Some Env.
+Proof.
+  move => [/=Hsub [_ /heap_bij_merge_prog_eq_i Hprog]] Hbija Hbij'.
+  destruct (decide (pi ∈ hb_shared_i bijb)) as [Hin|Hin]; [|naive_solver].
+  rewrite elem_of_hb_shared_i in Hin. move: Hin => [ps ?].
+  move: (Hsub ps pii). rewrite heap_bij_merge_shared => /(_ _)/hb_disj.
+  naive_solver.
+Qed.
+
+Lemma heap_bij_merge_extend_prog_i bija bijb bij' pi pii:
+  heap_bij_extend Env (heap_bij_merge bija bijb) bij' →
+  hb_players_i bija !! pii = Some Prog →
+  hb_bij bij' !! pi ≠ Some (HBShared pii).
+Proof. move => [/=Hsub [_ /heap_bij_merge_prog_eq_i Hprog]] Hbija /hb_disj Hbij'. naive_solver. Qed.
 
 (** ** val_in_bij *)
-Definition val_in_bij (bij : gset (prov * prov)) (v1 v2 : val) : Prop :=
+Definition val_in_bij (bij : heap_bij) (v1 v2 : val) : Prop :=
   match v1, v2 with
   | ValNum n1, ValNum n2 => n1 = n2
   | ValBool b1, ValBool b2 => b1 = b2
-  | ValLoc l1, ValLoc l2 => (l1.1, l2.1) ∈ bij /\ l1.2 = l2.2
+  | ValLoc l1, ValLoc l2 => hb_bij bij !! l2.1 = Some (HBShared l1.1) /\ l1.2 = l2.2
   | _, _ => False
   end.
 
@@ -85,10 +407,22 @@ Lemma val_in_bij_mono bij bij' v1 v2:
   val_in_bij bij v1 v2 →
   bij ⊆ bij' →
   val_in_bij bij' v1 v2.
-Proof. destruct v1, v2 => //=. set_solver. Qed.
+Proof. destruct v1, v2 => //=. bij_solver. Qed.
+
+Lemma val_in_bij_merge bija bijb vii vs :
+  val_in_bij (heap_bij_merge bija bijb) vii vs ↔ ∃ vi,
+      val_in_bij bija vii vi ∧ val_in_bij bijb vi vs.
+Proof.
+   split.
+   - destruct vii, vs => //=. { by eexists (ValNum _). } { by eexists (ValBool _). }
+     move => [/heap_bij_merge_shared[?[??]] ?].
+     eexists (ValLoc (_, _)) => /=. naive_solver.
+   - move => [vi [??]]. destruct vii, vi, vs => //; simplify_eq/= => //.
+     split; [|naive_solver congruence]. apply heap_bij_merge_shared. naive_solver.
+Qed.
 
 (** ** expr_in_bij *)
-Fixpoint expr_in_bij (bij : gset (prov * prov)) (e1 e2 : expr) {struct e1} : Prop :=
+Fixpoint expr_in_bij (bij : heap_bij) (e1 e2 : expr) {struct e1} : Prop :=
   match e1, e2 with
   | Var v, Var v' => v = v'
   | Val v, Val v' => val_in_bij bij v v'
@@ -169,7 +503,7 @@ Proof.
 Qed.
 
 (** ** ectx_in_bij *)
-Definition ectx_item_in_bij (bij : gset (prov * prov)) (Ki Ki' : expr_ectx) : Prop :=
+Definition ectx_item_in_bij (bij : heap_bij) (Ki Ki' : expr_ectx) : Prop :=
   match Ki, Ki' with
   | BinOpLCtx op e2, BinOpLCtx op' e2' => op = op' ∧ expr_in_bij bij e2 e2'
   | BinOpRCtx v1 op, BinOpRCtx v1' op' => op = op' ∧ val_in_bij bij v1 v1'
@@ -186,7 +520,7 @@ Definition ectx_item_in_bij (bij : gset (prov * prov)) (Ki Ki' : expr_ectx) : Pr
   | _, _ => False
   end.
 
-Definition ectx_in_bij (bij : gset (prov * prov)) (K1 K2 : list expr_ectx) : Prop :=
+Definition ectx_in_bij (bij : heap_bij) (K1 K2 : list expr_ectx) : Prop :=
   Forall2 (ectx_item_in_bij bij) K1 K2.
 
 Lemma ectx_item_in_bij_mono bij bij' K1 K2:
@@ -276,9 +610,9 @@ Proof.
 Qed.
 
 (** *** heap_in_bij *)
-Definition heap_in_bij (bij : gset (prov * prov)) (h h' : heap_state) : Prop :=
+Definition heap_in_bij (bij : heap_bij) (h h' : heap_state) : Prop :=
   ∀ p1 p2 o,
-  (p1, p2) ∈ bij →
+  hb_bij bij !! p2 = Some (HBShared p1) →
 
   (is_Some (h.(h_heap) !! (p1, o)) ↔ is_Some (h'.(h_heap) !! (p2, o)))
   /\
@@ -287,10 +621,35 @@ Definition heap_in_bij (bij : gset (prov * prov)) (h h' : heap_state) : Prop :=
   h'.(h_heap) !! (p2, o) = Some v2 →
   val_in_bij bij v1 v2.
 
+Lemma heap_in_bij_mono bij bij' h h':
+  heap_in_bij bij h h' →
+  bij' ⊆ bij →
+  bij ⊆ bij' →
+  heap_in_bij bij' h h'.
+Proof.
+  move => Hh Hsub1 Hsub2 ????. split; [by apply Hh, Hsub1|].
+  move => ????. apply: val_in_bij_mono; [|done]. eapply Hh; [|done..].
+  by apply Hsub1.
+Qed.
+
+Lemma heap_in_bij_merge bija bijb hii hi hs :
+  heap_in_bij bija hii hi →
+  heap_in_bij bijb hi hs →
+  heap_in_bij (heap_bij_merge bija bijb) hii hs.
+Proof.
+  move => Hha Hhb pii ps o /heap_bij_merge_shared[pi[??]].
+  split. { etrans; [by apply Hha| by eapply Hhb]. }
+  move => ????. apply val_in_bij_merge.
+  move: (Hha pii pi o) => [//|??].
+  have [??]: is_Some (h_heap hi !! (pi, o)) by naive_solver.
+  move: (Hhb pi ps o) => [//|??].
+  naive_solver.
+Qed.
+
 Lemma heap_in_bij_alive bij h1 h2 l1 l2:
   heap_in_bij bij h1 h2 →
   heap_alive h2 l2 →
-  (l1.1, l2.1) ∈ bij →
+  hb_bij bij !! l2.1 = Some (HBShared l1.1) →
   l1.2 = l2.2 →
   heap_alive h1 l1.
 Proof.
@@ -301,7 +660,7 @@ Qed.
 Lemma heap_in_bij_lookup bij h1 h2 l1 l2 v:
   h_heap h2 !! l2 = Some v →
   heap_in_bij bij h1 h2 →
-  (l1.1, l2.1) ∈ bij →
+  hb_bij bij !! l2.1 = Some (HBShared l1.1) →
   l1.2 = l2.2 →
   ∃ v', h_heap h1 !! l1 = Some v' ∧ val_in_bij bij v' v.
 Proof.
@@ -312,88 +671,89 @@ Proof.
 Qed.
 
 Lemma heap_in_bij_update bij h1 h2 l1 l2 v1 v2:
-  heap_in_bij (hb_bij bij) h1 h2 →
-  val_in_bij (hb_bij bij) v1 v2 →
-  (l1.1, l2.1) ∈ (hb_bij bij) →
+  heap_in_bij bij h1 h2 →
+  val_in_bij bij v1 v2 →
+  hb_bij bij !! l2.1 = Some (HBShared l1.1) →
   l1.2 = l2.2 →
-  heap_in_bij (hb_bij bij) (heap_update h1 l1 v1) (heap_update h2 l2 v2).
+  heap_in_bij bij (heap_update h1 l1 v1) (heap_update h2 l2 v2).
 Proof.
   move => Hbij ???. destruct l1 as [p1 ?], l2 as [p2 o]; simplify_eq/=.
-  move => p1' p2' o' /=?. have : p1 = p1' ↔ p2 = p2' by apply: hb_iff.
+  move => p1' p2' o' /=?.
   split.
   - rewrite !lookup_alter_is_Some. by apply Hbij.
-  - move => ?? /lookup_alter_Some[[?[?[??]]]|[??]] /lookup_alter_Some[[?[?[??]]]|[??]]; simplify_eq.
-    all: try by eapply Hbij. all: naive_solver.
+  - move => ?? /lookup_alter_Some[[?[?[??]]]|[??]] /lookup_alter_Some[[?[?[??]]]|[??]]; simplify_bij.
+    all: try by eapply Hbij. all: try naive_solver.
 Qed.
 
 Lemma heap_in_bij_update_r bij h1 h2 l2 v2:
   heap_in_bij bij h1 h2 →
-  l2.1 ∉ set_map (D:=gset _) snd bij →
+  (∀ p, hb_bij bij !! l2.1 = Some (HBShared p) → False) →
   heap_in_bij bij h1 (heap_update h2 l2 v2).
 Proof.
   move => Hbij Hin ? ??? /=.
   rewrite !lookup_alter_ne. 1: by apply Hbij.
-  contradict Hin; subst => /=. apply elem_of_map.
-  eexists (_, _). naive_solver.
+  move => ?; subst => /=. by apply: Hin.
 Qed.
 
-Lemma heap_in_bij_alloc l1 l2 hi hs n bij H1 H2:
-  heap_in_bij (hb_bij bij) hi hs →
+(*
+Lemma heap_in_bij_alloc l1 l2 hi hs n bij H1:
+  heap_in_bij bij hi hs →
   heap_is_fresh hi l1 →
   heap_is_fresh hs l2 →
-  heap_in_bij (hb_bij (heap_bij_add_loc l1.1 l2.1 bij H1 H2)) (heap_alloc hi l1 n) (heap_alloc hs l2 n).
+  (∀ p, hb_bij bij !! l2.1 = Some (HBShared p) → False) →
+  heap_in_bij (heap_bij_add_shared l1.1 l2.1 bij H1) (heap_alloc hi l1 n) (heap_alloc hs l2 n).
 Proof.
-  move => /= Hbij [Hi1 ?] [Hi2 ?] p1 p2 o /= /elem_of_union[?|?].
-  - set_unfold; simplify_eq. destruct l1 as [p1 ?], l2 as [p2 ?]; simplify_eq/=.
+  move => /= Hbij [Hi1 ?] [Hi2 ?] ?  p1 p2 o /= /lookup_insert_Some[[??]|[??]]; simplify_eq.
+  - destruct l1 as [p1 ?], l2 as [p2 ?]; simplify_eq/=.
     rewrite !lookup_union_l'.
     2: { apply eq_None_ne_Some => ??. apply Hi2. by apply: (heap_wf _ (_, _)). }
     2: { apply eq_None_ne_Some => ??. apply Hi1. by apply: (heap_wf _ (_, _)). }
     split.
-    + rewrite !list_to_map_lookup_is_Some. f_equiv => ?. rewrite !elem_of_list_fmap. f_equiv => ?. naive_solver.
+    + rewrite !list_to_map_lookup_is_Some. f_equiv => ?. rewrite !elem_of_list_fmap.
+      f_equiv => ?. naive_solver.
     + move => ?? /(elem_of_list_to_map_2 _ _ _)/elem_of_list_fmap[?[??]].
       move => /(elem_of_list_to_map_2 _ _ _)/elem_of_list_fmap[?[??]]. by simplify_eq/=.
-  - have ? : p1 ≠ l1.1 by contradict H1; set_unfold; eexists (_, _); naive_solver.
-    have ? : p2 ≠ l2.1 by contradict H2; set_unfold; left; left; eexists (_, _); naive_solver.
+  - have ? : p1 ≠ l1.1. { contradict H1. apply elem_of_hb_shared_i. naive_solver. }
     have [Hbij1 Hbij2]:= Hbij p1 p2 o ltac:(set_solver).
     rewrite !lookup_union_r.
     2, 3: apply not_elem_of_list_to_map_1;
         move => /elem_of_list_fmap[[[??]?] [?/elem_of_list_fmap[?[??]]]]; simplify_eq/=.
-    split; [done|] => *. apply: val_in_bij_mono; [naive_solver|]. set_solver.
+    split; [done|] => *. apply: val_in_bij_mono; [naive_solver|].
+    move => ??/=?. apply lookup_insert_Some. naive_solver.
 Qed.
-
+*)
 Lemma heap_in_bij_alloc_r l2 hi hs n bij:
   heap_in_bij bij hi hs →
-  l2.1 ∉ set_map (D:=gset _) snd bij →
+  (∀ p, hb_bij bij !! l2.1 = Some (HBShared p) → False) →
   heap_in_bij bij hi (heap_alloc hs l2 n).
 Proof.
   move => /= Hbij Hin ???? /=. rewrite lookup_union_r. 1: by apply Hbij.
   apply not_elem_of_list_to_map_1. contradict Hin.
   move: Hin => /elem_of_list_fmap[[??][?/elem_of_list_fmap[?[??]]]]; simplify_eq/=.
-  apply elem_of_map. eexists (_, _). naive_solver.
+  naive_solver.
 Qed.
 
 Lemma heap_in_bij_free hi hs l1 l2 bij:
-  heap_in_bij (hb_bij bij) hi hs →
-  (l1.1, l2.1) ∈ hb_bij bij →
-  heap_in_bij (hb_bij bij) (heap_free hi l1) (heap_free hs l2).
+  heap_in_bij bij hi hs →
+  hb_bij bij !! l2.1 = Some (HBShared l1.1) →
+  heap_in_bij bij (heap_free hi l1) (heap_free hs l2).
 Proof.
   move => Hbij Hin p1 p2 o /=?.
   have [Hbij1 Hbij2]:= Hbij p1 p2 o ltac:(done).
-  have ?: p1 = l1.1 ↔ p2 = l2.1 by apply: hb_iff.
   split.
   - rewrite !map_filter_lookup /=. destruct (h_heap hi !! (p1, o)), (h_heap hs !! (p2, o)) => //=.
-    all: repeat case_option_guard => //; naive_solver.
+    all: repeat case_option_guard => //; simplify_bij; naive_solver.
   - move => ??. rewrite !map_filter_lookup => /bind_Some[?[??]] /bind_Some[?[??]].
     repeat case_option_guard => //; naive_solver.
 Qed.
 
 Lemma heap_in_bij_free_r hi hs l2 bij:
   heap_in_bij bij hi hs →
-  l2.1 ∉ set_map (D:=gset _) snd bij →
+  (∀ p, hb_bij bij !! l2.1 = Some (HBShared p) → False) →
   heap_in_bij bij hi (heap_free hs l2).
 Proof.
   move => /= Hbij Hin ???? /=. rewrite map_filter_lookup_true. 1: by apply Hbij.
-  move => ??. contradict Hin. apply elem_of_map. eexists (_, _). naive_solver.
+  naive_solver.
 Qed.
 
 (** *** heap_preserved *)
@@ -429,25 +789,25 @@ Proof.
   move => Hp ? p o /=?. rewrite lookup_alter_ne; [by eapply Hp|set_solver].
 Qed.
 
-Lemma heap_preserved_bij_env p1 p2 l v he hp bij:
-  (p1, p2) ∈ hb_bij bij →
-  l.1 = p2 →
-  heap_preserved (hb_env bij) he hp →
-  heap_preserved (hb_env bij) he (heap_update hp l v).
+Lemma heap_preserved_player pl pi ps l v he hp bij:
+  hb_bij bij !! ps = Some (HBShared pi) →
+  l.1 = ps →
+  heap_preserved (hb_player_s pl bij) he hp →
+  heap_preserved (hb_player_s pl bij) he (heap_update hp l v).
 Proof.
   move => ???. apply heap_preserved_update_r; [done|].
-  move => ?. have := hb_disj_env bij. apply; [done|]. apply elem_of_map. by eexists (_, _).
+  move => /elem_of_hb_player_s?. naive_solver.
 Qed.
 
-Lemma heap_preserved_bij_env_free p1 p2 l he hp bij:
-  (p1, p2) ∈ hb_bij bij →
-  l.1 = p2 →
-  heap_preserved (hb_env bij) he hp →
-  heap_preserved (hb_env bij) he (heap_free hp l).
+Lemma heap_preserved_bij_player_free pl pi ps l he hp bij:
+  hb_bij bij !! ps = Some (HBShared pi) →
+  l.1 = ps →
+  heap_preserved (hb_player_s pl bij) he hp →
+  heap_preserved (hb_player_s pl bij) he (heap_free hp l).
 Proof.
-  move => ?? Hp p o /=?. rewrite map_filter_lookup. etrans; [by apply Hp|].
-  destruct (h_heap hp !! (p, o)) => //=. case_option_guard => //.
-  exfalso. have := hb_disj_env bij. apply; [done|]. apply elem_of_map. eexists (_, _). naive_solver.
+  move => ?? Hp p' o /= Hin. rewrite map_filter_lookup. etrans; [by apply Hp|].
+  destruct (h_heap hp !! (p', o)) => //=. case_option_guard => //.
+  exfalso. move: Hin => /elem_of_hb_player_s?. naive_solver.
 Qed.
 
 Lemma heap_preserved_alloc_r l n he hp bij:
@@ -466,56 +826,586 @@ Lemma heap_preserved_free_r l he hp bij:
   heap_preserved bij he (heap_free hp l).
 Proof. move => Hni Hp p o /= ?. rewrite map_filter_lookup_true; [by apply Hp|]. set_solver. Qed.
 
+(** * imp_heap_bij module *)
 Record imp_heap_bij_state := ImpHeapBij {
   ihb_bij : heap_bij;
-  (* last seen heap *)
-  ihb_heap : heap_state;
+  (* last seen heaps *)
+  ihb_heap_i : heap_state;
+  ihb_heap_s : heap_state;
 }.
 Add Printing Constructor imp_heap_bij_state.
 
 Definition imp_heap_bij_pre (e : imp_event) (s : imp_heap_bij_state) : prepost (imp_event * imp_heap_bij_state) unitUR :=
-  let ho := heap_of_event e.2 in
+  let hi := heap_of_event e.2 in
+  pp_quant $ λ bij',
+  pp_quant $ λ vss,
+  pp_quant $ λ hs,
+  pp_prop (heap_bij_extend Env s.(ihb_bij) bij') $
+  pp_prop (dom _ (hb_bij bij') ⊆ h_provs hs) $
+  pp_prop (hb_provs_i bij' ⊆ h_provs hi) $
+  pp_prop (Forall2 (val_in_bij bij') (vals_of_event e.2) vss) $
+  pp_prop (heap_in_bij bij' hi hs) $
+  pp_prop (heap_preserved (hb_player_s Prog bij') s.(ihb_heap_s) hs) $
+  pp_prop (heap_preserved (hb_player_i Prog bij') s.(ihb_heap_i) hi) $
+  pp_end ((e.1, event_set_vals_heap e.2 vss hs), ImpHeapBij bij' hi hs).
+
+Definition imp_heap_bij_post (e : imp_event) (s : imp_heap_bij_state) : prepost (imp_event * imp_heap_bij_state) unitUR :=
+  let hs := heap_of_event e.2 in
   pp_quant $ λ bij',
   pp_quant $ λ vsi,
   pp_quant $ λ hi,
-  pp_prop (heap_bij_extend Env s.(ihb_bij) bij') $
-  (* TODO: should we also have the following for hi? We don't need it so far... *)
-  pp_prop (set_map fst (hb_bij bij') ⊆ h_provs ho) $
-  pp_prop (Forall2 (val_in_bij (hb_bij bij')) (vals_of_event e.2) vsi) $
-  pp_prop (heap_in_bij (hb_bij bij') ho hi) $
-  pp_prop (heap_preserved (hb_prog bij') s.(ihb_heap) hi) $
-  pp_end ((e.1, event_set_vals_heap e.2 vsi hi), ImpHeapBij bij' hi).
-
-Definition imp_heap_bij_post (e : imp_event) (s : imp_heap_bij_state) : prepost (imp_event * imp_heap_bij_state) unitUR :=
-  let hi := heap_of_event e.2 in
-  pp_quant $ λ bij',
-  pp_quant $ λ vso,
-  pp_quant $ λ ho,
   pp_prop (heap_bij_extend Prog s.(ihb_bij) bij') $
-  (* TODO: should we also have the following for hi? We don't need it so far... *)
-  pp_prop (set_map fst (hb_bij bij') ⊆ h_provs ho) $
-  pp_prop (Forall2 (val_in_bij (hb_bij bij')) vso (vals_of_event e.2)) $
-  pp_prop (heap_in_bij (hb_bij bij') ho hi) $
-  pp_prop (heap_preserved (hb_env bij') s.(ihb_heap) hi) $
+  pp_prop (dom _ (hb_bij bij') ⊆ h_provs hs) $
+  pp_prop (hb_provs_i bij' ⊆ h_provs hi) $
+  pp_prop (Forall2 (val_in_bij bij') vsi (vals_of_event e.2)) $
+  pp_prop (heap_in_bij bij' hi hs) $
+  pp_prop (heap_preserved (hb_player_i Env bij') s.(ihb_heap_i) hi) $
+  pp_prop (heap_preserved (hb_player_s Env bij') s.(ihb_heap_s) hs) $
   pp_remove True $
-  pp_end ((e.1, event_set_vals_heap e.2 vso ho), ImpHeapBij bij' hi).
+  pp_end ((e.1, event_set_vals_heap e.2 vsi hi), ImpHeapBij bij' hi hs).
 
 Definition imp_heap_bij (m : module imp_event) : module imp_event :=
   mod_prepost imp_heap_bij_pre imp_heap_bij_post m.
 
 Definition initial_imp_heap_bij_state (m : module imp_event) (σ : m.(m_state)) :=
-  (@SMFilter imp_event, σ, (@PPOutside imp_event imp_event, ImpHeapBij ∅ initial_heap_state, (True%I : uPred unitUR))).
+  (@SMFilter imp_event, σ, (@PPOutside imp_event imp_event, ImpHeapBij ∅ initial_heap_state initial_heap_state, (True%I : uPred unitUR))).
+
+(** * vertical compositionality *)
+(** ** map values and heaps through bij *)
+(** *** val_through_bij *)
+Definition val_through_bij (bij : heap_bij) (vs : val) : val :=
+  match vs with
+  | ValLoc l => ValLoc (if hb_bij bij !! l.1 is Some (HBShared p) then p else inhabitant, l.2)
+  | _ => vs
+  end.
+
+Lemma val_through_in_bij bij vs:
+  (∀ l, vs = ValLoc l → ∃ p, hb_bij bij !! l.1 = Some (HBShared p)) →
+  val_in_bij bij (val_through_bij bij vs) vs.
+Proof. move => ?. destruct vs => //=. case_match; naive_solver. Qed.
+
+(** *** heap_through_bij *)
+Program Definition heap_through_bij (bij : heap_bij) (h : heap_state) : heap_state :=
+  Heap (list_to_map $ omap (OMap:=list_omap) (λ '(l, v), if hb_bij bij !! l.1 is Some (HBShared p) then
+         Some ((p, l.2), val_through_bij bij v) else None) (map_to_list (h_heap h))) (hb_shared_i bij) _.
+Next Obligation.
+  move => ??. apply bool_decide_spec. move => ? /elem_of_map[?[?/elem_of_dom]]. subst.
+  rewrite list_to_map_lookup_is_Some => -[?]. rewrite elem_of_list_omap => -[[[??]?]]/=[??].
+  repeat case_match; simplify_eq. rewrite elem_of_hb_shared_i. naive_solver.
+Qed.
+
+Lemma heap_through_bij_provs bij h :
+  h_provs (heap_through_bij bij h) = hb_shared_i bij.
+Proof. done. Qed.
+
+Lemma heap_through_bij_Some bij h pi o vi:
+  h_heap (heap_through_bij bij h) !! (pi, o) = Some vi ↔
+    ∃ ps vs, hb_bij bij !! ps = Some (HBShared pi) ∧ h_heap h !! (ps, o) = Some vs ∧ vi = val_through_bij bij vs.
+Proof.
+  simpl. rewrite -elem_of_list_to_map. 2: {
+    rewrite list_fmap_omap. apply NoDup_omap_2_strong; [|apply NoDup_map_to_list].
+    move => [[??]?] [[??]?] [??] /=.
+    move => /elem_of_map_to_list ?/elem_of_map_to_list? /fmap_Some[[??][??]] /fmap_Some[[??][??]].
+    by repeat case_match; simplify_eq/=; simplify_bij.
+  }
+  rewrite elem_of_list_omap.
+  split.
+  - move => [[[??]?]]. rewrite elem_of_map_to_list => ?. repeat case_match => //; naive_solver.
+  - move => ?. destruct_all?. eexists (_,_,_). rewrite elem_of_map_to_list. split; [done|].
+    by simplify_option_eq.
+Qed.
+Opaque heap_through_bij.
+
+Lemma heap_through_bij_is_Some bij h pi o:
+  is_Some (h_heap (heap_through_bij bij h) !! (pi, o)) ↔
+          ∃ ps, hb_bij bij !! ps = Some (HBShared pi) ∧ is_Some (h_heap h !! (ps, o)).
+Proof. rewrite /is_Some. setoid_rewrite heap_through_bij_Some. naive_solver. Qed.
+
+Lemma heap_through_bij_is_Some' bij h pi ps o:
+  hb_bij bij !! ps = Some (HBShared pi) →
+  is_Some (h_heap (heap_through_bij bij h) !! (pi, o)) ↔ is_Some (h_heap h !! (ps, o)).
+Proof.
+  move => ?. rewrite heap_through_bij_is_Some. split; [|naive_solver].
+  move => [p'[??]]. by simplify_bij.
+Qed.
+
+(** ** splitting bij' into two parts *)
+Lemma fresh_map_learn bij' bijb (X : gset prov) ps pi:
+  fresh_map (hb_shared_s bij' ∖ hb_shared_s bijb) X !! ps = Some pi →
+  (∃ pii, hb_bij bij' !! ps = Some (HBShared pii) ∧ ∀ pi', hb_bij bijb !! ps ≠ Some (HBShared pi'))
+   ∧ pi ∉ X.
+Proof. move => /(fresh_map_lookup_Some _ _ _ _)[/elem_of_difference ]. rewrite !elem_of_hb_shared_s. naive_solver. Qed.
+Ltac fresh_map_learn :=
+  repeat match goal with
+         | H : fresh_map (hb_shared_s _ ∖ hb_shared_s _) _ !! _ = Some _ |- _ =>
+             learn_hyp (fresh_map_learn _ _ _ _ _ H)
+         end.
+
+Definition heap_bij_splitb_bij (X : gset prov) (bijb bij' : heap_bij) :=
+  (gset_to_gmap (HBOwned Prog) (hb_player_s Prog bijb) ∪
+   (HBShared <$> (hb_shared bijb ∪ fresh_map (hb_shared_s bij' ∖ hb_shared_s bijb) X)) ∪
+   hb_bij bij').
+
+Lemma heap_bij_splitb_bij_prog X bijb bija bij' ps :
+  hb_player_s Prog (heap_bij_merge bija bijb) = hb_player_s Prog bij' →
+  heap_bij_splitb_bij X bijb bij' !! ps = Some (HBOwned Prog) ↔ ps ∈ hb_player_s Prog bijb.
+Proof.
+  move => /heap_bij_merge_prog_eq_s Hprog.
+  rewrite elem_of_hb_player_s /heap_bij_splitb_bij !lookup_union_Some_raw lookup_union_None lookup_fmap.
+  rewrite fmap_None fmap_Some lookup_union_None hb_shared_lookup.
+  rewrite !lookup_gset_to_gmap_Some lookup_gset_to_gmap_None elem_of_hb_player_s.
+  split; [|naive_solver]. move => ?. destruct_all? => //. naive_solver (simplify_option_eq).
+Qed.
+
+Lemma heap_bij_splitb_bij_env X bijb bija bij' ps :
+  heap_bij_extend Env (heap_bij_merge bija bijb) bij' →
+  hb_player_s Env bija = ∅ →
+  heap_bij_splitb_bij X bijb bij' !! ps = Some (HBOwned Env) ↔ ps ∈ hb_player_s Env bij'.
+Proof.
+  move => ??.
+  rewrite elem_of_hb_player_s /heap_bij_splitb_bij !lookup_union_Some_raw lookup_union_None lookup_fmap.
+  rewrite fmap_None fmap_Some lookup_union_None hb_shared_lookup.
+  rewrite !lookup_gset_to_gmap_Some lookup_gset_to_gmap_None elem_of_hb_player_s.
+  split => ?; destruct_all?; simplify_option_eq => //.
+  right.
+  rewrite fresh_map_lookup_None not_elem_of_difference elem_of_hb_shared_s.
+  destruct (hb_bij bijb !! ps) eqn:? => /=; [|naive_solver].
+  efeed pose proof heap_bij_merge_extend_env; [done..|]; simplify_eq. naive_solver.
+Qed.
+
+Lemma heap_bij_splitb_bij_bij X bijb bija bij' ps pi:
+  heap_bij_extend Env (heap_bij_merge bija bijb) bij' →
+  heap_bij_splitb_bij X bijb bij' !! ps = Some (HBShared pi) ↔
+   hb_bij bijb !! ps = Some (HBShared pi) ∨ fresh_map (hb_shared_s bij' ∖ hb_shared_s bijb) X !! ps = Some pi.
+Proof.
+  move => [/=Hsub [Hprog ?]].
+  rewrite /heap_bij_splitb_bij !lookup_union_Some_raw lookup_union_None lookup_fmap.
+  rewrite fmap_None fmap_Some lookup_union_None.
+  rewrite !lookup_gset_to_gmap_Some lookup_gset_to_gmap_None elem_of_hb_player_s.
+  split => Heq; destruct_all?; simplify_eq.
+  - revert select ((_ ∪ _) !! _ = Some _) => /lookup_union_Some_raw.
+    rewrite hb_shared_lookup_Some. naive_solver.
+  - left. revert select (fresh_map _ _ !! _ = None) => /fresh_map_lookup_None. rewrite not_elem_of_difference.
+    revert select (hb_shared _ !! _ = None). rewrite hb_shared_lookup_None !elem_of_hb_shared_s. naive_solver.
+  - left. right. rewrite Heq. split; [done|]. eexists _. split; [|done].
+    apply lookup_union_Some_raw. rewrite hb_shared_lookup_Some. naive_solver.
+  - fresh_map_learn. move: Hprog => /heap_bij_merge_prog_eq_s?.
+    left. right. split; [naive_solver|].
+    eexists _. split; [|done]. apply lookup_union_Some_raw.
+    rewrite hb_shared_lookup_Some hb_shared_lookup_None. naive_solver.
+Qed.
+
+Program Definition heap_bij_splitb (X : gset prov) (bija bijb bij' : heap_bij)
+        (H1 : heap_bij_extend Env (heap_bij_merge bija bijb) bij')
+        (H2 : hb_provs_i bijb ⊆ X) : heap_bij :=
+  HeapBij (heap_bij_splitb_bij X bijb bij') (hb_players_i bijb) _ _.
+Next Obligation.
+  move => X bija bijb bij' Hex Hshared ps pi.
+  rewrite !heap_bij_splitb_bij_bij // => -[?|?]; [by apply: hb_disj|].
+  apply eq_None_ne_Some => ??.
+  have : (pi ∈ hb_provs_i bijb) by rewrite elem_of_hb_provs_i; naive_solver.
+  fresh_map_learn. set_solver.
+Qed.
+Next Obligation.
+  move => ????? Hp pi ??.
+  rewrite !heap_bij_splitb_bij_bij // => ??.
+  destruct_all?; simplify_bij.
+  - done.
+  - fresh_map_learn. move: (Hp pi). rewrite elem_of_hb_provs_i. naive_solver.
+  - fresh_map_learn. move: (Hp pi). rewrite elem_of_hb_provs_i. naive_solver.
+  - by apply: fresh_map_bij.
+Qed.
+
+
+(* Instead of trying to understand this definition, one can also look
+at the lemmas below. *)
+Definition heap_bij_splita_bij (X : gset prov) (bija bijb bij' : heap_bij) :=
+  (hb_bij bija ∪ list_to_map (
+     (λ '(ps, pi), (pi, HBShared $ if hb_bij bij' !! ps is Some (HBShared pii) then pii else inhabitant))
+       <$> (map_to_list (fresh_map (hb_shared_s bij' ∖ hb_shared_s bijb) X)))).
+
+Lemma heap_bij_splita_bij_None X bijb bija bij' pi :
+  heap_bij_splita_bij X bija bijb bij' !! pi = None ↔
+      hb_bij bija !! pi = None ∧ ∀ ps, fresh_map (hb_shared_s bij' ∖ hb_shared_s bijb) X !! ps ≠ Some pi.
+Proof.
+  rewrite lookup_union_None. f_equiv.
+  rewrite -not_elem_of_list_to_map -list_fmap_compose elem_of_list_fmap /=.
+  split.
+  - move => Hneg ??. apply Hneg. eexists (_, _) => /=. split; [done|]. by apply elem_of_map_to_list.
+  - move => ? [[??]/=[? /elem_of_map_to_list?]]. naive_solver.
+Qed.
+
+Lemma heap_bij_splita_bij_player X bijb bija bij' pi pl:
+  heap_bij_splita_bij X bija bijb bij' !! pi = Some (HBOwned pl) ↔ pi ∈ hb_player_s pl bija.
+Proof.
+  rewrite elem_of_hb_player_s /heap_bij_splita_bij !lookup_union_Some_raw. split; [|naive_solver].
+  move => [?//|[?]]. move => /(elem_of_list_to_map_2 _ _ _)/elem_of_list_fmap[[??]/=[??]]. simplify_eq.
+Qed.
+
+Lemma heap_bij_splita_bij_bij X bijb bija bij' pi pii:
+  dom _ (hb_bij bija) ⊆ X →
+  heap_bij_splita_bij X bija bijb bij' !! pi = Some (HBShared pii) ↔
+    hb_bij bija !! pi = Some (HBShared pii) ∨
+    ∃ ps, fresh_map (hb_shared_s bij' ∖ hb_shared_s bijb) X !! ps = Some pi
+          ∧ hb_bij bij' !! ps = Some (HBShared pii).
+Proof.
+  move => Hdom.
+  rewrite /heap_bij_splita_bij !lookup_union_Some_raw.
+  rewrite -elem_of_list_to_map.
+  2: { rewrite -list_fmap_compose. apply NoDup_fmap_2_strong; [|apply NoDup_map_to_list].
+       move => [??] [??] /elem_of_map_to_list? /elem_of_map_to_list? /= ?. subst.
+       f_equal. by apply: fresh_map_bij. }
+  rewrite elem_of_list_fmap.
+  split => ?; destruct_all?; simplify_eq; try naive_solver.
+  - revert select (_ ∈ map_to_list _) => /elem_of_map_to_list Hfresh. right. eexists _. split; [done|].
+    fresh_map_learn. destruct_all?. by simplify_option_eq.
+  - fresh_map_learn. destruct_all?; simplify_eq.
+    right. split. { apply eq_None_not_Some. rewrite -elem_of_dom. set_solver. }
+    eexists (_, _). rewrite elem_of_map_to_list. split; [|done]. by simplify_option_eq.
+Qed.
+
+Definition heap_bij_splita_players_i (bija bij' : heap_bij) : gmap prov player :=
+  gset_to_gmap Prog (hb_player_i Prog bija) ∪ gset_to_gmap Env (hb_player_i Env bij').
+
+Lemma heap_bij_splita_player_i_prog bija bij' pii :
+  heap_bij_splita_players_i bija bij' !! pii = Some Prog ↔ pii ∈ hb_player_i Prog bija.
+Proof. rewrite lookup_union_Some_raw !lookup_gset_to_gmap_Some. naive_solver. Qed.
+
+Lemma heap_bij_splita_player_i_env bija bijb bij' pii :
+  heap_bij_extend Env (heap_bij_merge bija bijb) bij' →
+  heap_bij_splita_players_i bija bij' !! pii = Some Env ↔ pii ∈ hb_player_i Env bij'.
+Proof.
+  move => [/=? [? /heap_bij_merge_prog_eq_i Hprog_i]].
+  rewrite lookup_union_Some_raw !lookup_gset_to_gmap_Some lookup_gset_to_gmap_None.
+  split; [naive_solver|]. rewrite !elem_of_hb_player_i => ?. split!.
+  move => ?. naive_solver.
+Qed.
+
+Program Definition heap_bij_splita (X : gset prov) (bija bijb bij' : heap_bij)
+        (H1 : dom _ (hb_bij bija) ⊆ X)
+        (H3 : heap_bij_extend Env (heap_bij_merge bija bijb) bij') :=
+  HeapBij (heap_bij_splita_bij X bija bijb bij') (heap_bij_splita_players_i bija bij') _ _.
+Next Obligation.
+  move => X bija bijb bij' HX Hextend pi pii.
+  rewrite !heap_bij_splita_bij_bij // => -[Hpi |[?[??]]].
+  - apply eq_None_ne_Some => -[].
+    + rewrite heap_bij_splita_player_i_prog elem_of_hb_player_i. move: Hpi => /hb_disj. naive_solver.
+    + rewrite heap_bij_splita_player_i_env // elem_of_hb_player_i.
+      by apply: heap_bij_merge_extend_env_i.
+  - apply eq_None_ne_Some => -[].
+    + rewrite heap_bij_splita_player_i_prog elem_of_hb_player_i => ?.
+      by apply: heap_bij_merge_extend_prog_i.
+    + rewrite heap_bij_splita_player_i_env // elem_of_hb_player_i.
+      apply eq_None_ne_Some_1. by apply: hb_disj.
+Qed.
+Next Obligation.
+  move => X bija bijb bij' HX [/=Hsub [Hprog_s Hprog_i]] pii pi pi'.
+  rewrite !heap_bij_splita_bij_bij // => ??. destruct_all?; simplify_bij.
+  - done.
+  - fresh_map_learn. destruct_all?; simplify_eq.
+    destruct (decide (pi' ∈ hb_shared_i bijb)) as [Hin'|Hin'].
+    + move: Hin'. rewrite elem_of_hb_shared_i => -[ps' ?]. move: (Hsub ps' pii).
+      rewrite heap_bij_merge_shared => /(_ ltac:(naive_solver)) ?. simplify_bij.
+      naive_solver.
+    + revert select (hb_bij bij' !! _ = Some _) => /hb_disj?.
+      have : hb_players_i bij' !! pii = Some Prog; [|naive_solver].
+      eapply heap_bij_merge_prog_eq_i; [done|]. naive_solver.
+  - fresh_map_learn. destruct_all?; simplify_eq.
+    destruct (decide (pi ∈ hb_shared_i bijb)) as [Hin'|Hin'].
+    + move: Hin'. rewrite elem_of_hb_shared_i => -[ps' ?]. move: (Hsub ps' pii).
+      rewrite heap_bij_merge_shared => /(_ ltac:(naive_solver)) ?. simplify_bij.
+      naive_solver.
+    + revert select (hb_bij bij' !! _ = Some _) => /hb_disj?.
+      have : hb_players_i bij' !! pii = Some Prog; [|naive_solver].
+      eapply heap_bij_merge_prog_eq_i; [done|]. naive_solver.
+  - done.
+Qed.
+
+Lemma heap_bij_merge_extend (X : gset prov) bijb bija bij':
+  heap_bij_extend Env (heap_bij_merge bija bijb) bij' →
+  hb_provs_i bijb ⊆ X →
+  dom (gset prov) (hb_bij bija) ⊆ X →
+  hb_player_s Env bija = ∅ →
+  ∃ bijb' bija', bij' = heap_bij_merge bija' bijb'
+    ∧ heap_bij_extend Env bija bija'
+    ∧ hb_player_s Env bija' = ∅
+    ∧ heap_bij_extend Env bijb bijb'
+    ∧ hb_provs_i bijb' ⊆ hb_shared_i bijb' ∪ X
+    ∧ dom (gset prov) (hb_bij bija') ⊆ hb_shared_i bijb' ∪ X
+    ∧ (∀ pi pii, hb_bij bija' !! pi = Some (HBShared pii) →
+         (∀ ps, hb_bij bijb' !! ps ≠ Some (HBShared pi)) →
+         hb_bij bija !! pi = Some (HBShared pii))
+    ∧ (∀ ps pi, hb_bij bijb' !! ps = Some (HBShared pi) →
+         (∀ pii, hb_bij bija' !! pi ≠ Some (HBShared pii)) →
+         hb_bij bijb !! ps = Some (HBShared pi))
+.
+Proof.
+  move => [/=Hextend1 [Hprog_s Hprog_i]] HX1 HX2 Hempty.
+  unshelve eexists (heap_bij_splitb X bija bijb bij' _ _); [done..|].
+  unshelve eexists (heap_bij_splita X bija bijb bij' _ _); [done..|].
+  split_and!.
+  - apply heap_bij_eq_parts. split.
+    + apply map_eq => ps. apply option_eq => pii.
+      rewrite !hb_shared_lookup_Some heap_bij_merge_shared /=.
+      setoid_rewrite heap_bij_splitb_bij_bij; [|done].
+      setoid_rewrite heap_bij_splita_bij_bij; [|done].
+      split.
+      * move => Hbij'. destruct (hb_bij bijb !! ps) as [[pi|[]]|] eqn:Hbijb.
+        -- eexists _. split; [naive_solver|]. left.
+           apply: heap_bij_merge_extend_a; [|done..]. done.
+        -- exfalso. move: Hprog_s => /heap_bij_merge_prog_eq_s. naive_solver.
+        -- have [??]: is_Some (fresh_map (hb_shared_s bij' ∖ hb_shared_s bijb) X !! ps).
+           { apply not_eq_None_Some. rewrite fresh_map_lookup_None. apply. apply elem_of_difference.
+             rewrite !elem_of_hb_shared_s. naive_solver. }
+           naive_solver.
+        -- have [??]: is_Some (fresh_map (hb_shared_s bij' ∖ hb_shared_s bijb) X !! ps).
+           { apply not_eq_None_Some. rewrite fresh_map_lookup_None. apply. apply elem_of_difference.
+             rewrite !elem_of_hb_shared_s. naive_solver. }
+           naive_solver.
+      * move => [? [Hor ?]].
+        destruct_all?; simplify_eq.
+        -- apply Hextend1. rewrite heap_bij_merge_shared. naive_solver.
+        -- exfalso. fresh_map_learn. destruct_all?. revert select (_ ∉ _). apply.
+           apply HX2. rewrite elem_of_dom. naive_solver.
+        -- exfalso. fresh_map_learn. destruct_all?. revert select (_ ∉ _). apply.
+           apply HX1. rewrite elem_of_hb_provs_i. naive_solver.
+        -- have := fresh_map_bij _ _ ps0 ps _ ltac:(done) ltac:(done). naive_solver.
+    + move => pl. split; apply set_eq => ?; destruct pl.
+      * rewrite - {1}Hprog_s !heap_bij_merge_player_s heap_bij_splitb_bij_prog ?elem_of_hb_player_s//.
+        setoid_rewrite heap_bij_splitb_bij_bij; [|done].
+        split => ?; destruct_all?; simplify_eq; try naive_solver.
+        -- right. eexists _. split; [naive_solver|].
+           apply default_eq_Some' => -[?|?] /=.
+           ++ rewrite heap_bij_splita_bij_bij // => -[?|?]; simplify_option_eq. destruct_all?.
+              exfalso. fresh_map_learn. destruct_all?. revert select (_ ∉ _). apply.
+              apply HX1. rewrite elem_of_hb_provs_i. naive_solver.
+           ++ rewrite heap_bij_splita_bij_player elem_of_hb_player_s => ?. by simplify_option_eq.
+        -- right. eexists _. split; [done|]. rewrite default_eq_Some' /= => y.
+           revert select (default _ _ = _). rewrite default_eq_Some' => /(_ y). move: y => -[?|?].
+           ++ rewrite heap_bij_splita_bij_bij //. naive_solver.
+           ++ rewrite heap_bij_splita_bij_player elem_of_hb_player_s => ?. naive_solver.
+        -- simpl in *. unfold default in *. case_match as Hc => /=; simplify_eq/=.
+           ++ move: Hc. rewrite heap_bij_splita_bij_player elem_of_hb_player_s => ?.
+              exfalso. fresh_map_learn. destruct_all?. revert select (_ ∉ _). apply.
+              apply HX2. rewrite elem_of_dom. naive_solver.
+           ++ move: Hc => /heap_bij_splita_bij_None. naive_solver.
+      * rewrite !heap_bij_merge_player_s heap_bij_splitb_bij_env //=.
+        setoid_rewrite heap_bij_splitb_bij_bij; [|done].
+        setoid_rewrite default_eq_neq => //.
+        setoid_rewrite heap_bij_splita_bij_player.
+        rewrite Hempty. set_solver.
+      * rewrite - {1}Hprog_i !heap_bij_merge_player_i /= heap_bij_splita_player_i_prog elem_of_hb_player_i.
+        setoid_rewrite heap_bij_splita_bij_bij; [|done].
+        split => ?; destruct_all?; simplify_eq; try by left.
+        -- right. split!; [by left|]. rewrite elem_of_hb_shared_i => /= -[?].
+           rewrite heap_bij_splitb_bij_bij // => -[?|?].
+           ++ revert select (_ ∉ _). apply. rewrite elem_of_hb_shared_i. naive_solver.
+           ++ fresh_map_learn. destruct_all?; simplify_eq. revert select (_ ∉ _). apply. apply HX2.
+              rewrite elem_of_dom. naive_solver.
+        -- right. split!; [done|] => Hb. revert select (_ ∉ _). apply.
+           move: Hb. rewrite !elem_of_hb_shared_i => -[??]. eexists _.
+           rewrite heap_bij_splitb_bij_bij //. naive_solver.
+        -- exfalso. revert select (_ ∉ _). apply. rewrite !elem_of_hb_shared_i. eexists _.
+           rewrite heap_bij_splitb_bij_bij //. naive_solver.
+      * rewrite !heap_bij_merge_player_i !elem_of_hb_player_i /= heap_bij_splita_player_i_env //.
+        rewrite elem_of_hb_player_i. naive_solver.
+  - split => /=; [|split].
+    + move => ?? /=. rewrite heap_bij_splita_bij_bij //. naive_solver.
+    + apply set_eq => p. by rewrite !elem_of_hb_player_s /= heap_bij_splita_bij_player elem_of_hb_player_s.
+    + apply set_eq => p. by rewrite !elem_of_hb_player_i /= heap_bij_splita_player_i_prog elem_of_hb_player_i.
+  - apply set_eq => p. rewrite elem_of_hb_player_s /= heap_bij_splita_bij_player. set_solver.
+  - split => /=; [|split].
+    + move => ?? /=. rewrite heap_bij_splitb_bij_bij //. naive_solver.
+    + apply set_eq => p. by rewrite !elem_of_hb_player_s /= heap_bij_splitb_bij_prog // elem_of_hb_player_s.
+    + apply set_eq => p. by rewrite !elem_of_hb_player_i /=.
+  - move => ?. rewrite elem_of_union. rewrite elem_of_hb_provs_i/= => -[[??]|[?]].
+    { right. apply HX1. rewrite elem_of_hb_provs_i. naive_solver. }
+    rewrite heap_bij_splitb_bij_bij // => -[?|?].
+    { right. apply HX1. rewrite elem_of_hb_provs_i. naive_solver. }
+    rewrite elem_of_hb_shared_i/=.
+    setoid_rewrite heap_bij_splitb_bij_bij; [|done]. naive_solver.
+  - move => ? /=/elem_of_dom[x ]. rewrite elem_of_union elem_of_hb_shared_i /=.
+    setoid_rewrite heap_bij_splitb_bij_bij; [|done].
+    destruct x.
+    + rewrite heap_bij_splita_bij_bij //. move => ?. destruct_all?. 2: naive_solver.
+      right. apply HX2. by apply elem_of_dom.
+    + rewrite heap_bij_splita_bij_player elem_of_hb_player_s. right. apply HX2. by apply elem_of_dom.
+  - move => ?? /=. rewrite heap_bij_splita_bij_bij //. setoid_rewrite heap_bij_splitb_bij_bij; [|done].
+    naive_solver.
+  - move => ?? /=. rewrite heap_bij_splitb_bij_bij //. setoid_rewrite heap_bij_splita_bij_bij; [|done].
+    move => [//|?]. fresh_map_learn; destruct_all?. naive_solver.
+Qed.
+
+(** ** proof of vertical compositionality *)
+Local Ltac split_solve :=
+  match goal with
+  | _ => rewrite event_set_vals_heap_idemp
+  | |- event_set_vals_heap _ _ _ = event_set_vals_heap _ _ _ => reflexivity
+  end.
+Local Ltac split_tac ::=
+  repeat (original_split_tac; try split_solve).
+
+Lemma imp_heap_bij_vertical m σ `{!VisNoAll m}:
+  trefines (MS (imp_heap_bij (imp_heap_bij m))
+               (initial_imp_heap_bij_state (imp_heap_bij m) (initial_imp_heap_bij_state m σ)))
+           (MS (imp_heap_bij m)
+               (initial_imp_heap_bij_state m σ))
+.
+Proof.
+  unshelve apply: mod_prepost_combine. {
+    exact (λ pl '(ImpHeapBij bija hia hsa) '(ImpHeapBij bijb hib hsb) '(ImpHeapBij bij hi hs) _ _ _,
+    hb_player_s Env bija = ∅
+    ∧ bij = heap_bij_merge bija bijb
+    ∧ hsb = hs
+    ∧ hia = hi
+    ∧ hsa = hib
+    ∧
+    if pl is Env then
+      heap_in_bij bijb hsa hsb ∧
+      heap_in_bij bija hia hib ∧
+      dom (gset prov) (hb_bij bija) ⊆ h_provs hsa ∧
+      hb_provs_i bijb ⊆ h_provs hsa
+    else
+      True
+). }
+  { split!.
+    - apply set_eq => ?. rewrite elem_of_hb_player_s. set_solver.
+    - apply heap_bij_eq_parts => /=. split; [apply map_eq|move => pl; split; apply set_eq] => ?.
+      + rewrite !hb_shared_lookup heap_bij_merge_lookup. by simplify_map_eq.
+      + by rewrite elem_of_hb_player_s.
+      + by rewrite elem_of_hb_player_i.
+  }
+  all: move => [bija hia hsa] [bijb hib hsb] [bij hi hs] ??? e ? /=.
+  - move => bij' vs h' Hextend Hdh Hprovs Hvs Hh Hps Hpi.
+    destruct_all?; simplify_eq/=.
+    move: (Hextend) => /(heap_bij_merge_extend (h_provs hib))[//|//|//|bijb' [bija' [?[?[Hbij1e[?[?[??]]]]]]]]
+                      ; simplify_eq.
+    eexists _, (val_through_bij bijb' <$> vs),
+      (heap_merge (heap_restrict (heap_through_bij bijb' h') (λ p, p ∈ hb_shared_s bija'))
+                  (heap_restrict hib (λ x, x ∉ hb_shared_s bija' ∨ x ∉ hb_shared_i bijb'))).
+    split!; rewrite ?heap_of_event_event_set_vals_heap; split!; last done. all: split!.
+    + etrans; [|done]. move => ?. by rewrite heap_bij_merge_provs_i.
+    + rewrite Forall2_fmap_r. apply: Forall2_impl; [done|] => v_ii v_s /=.
+      destruct v_ii, v_s => //= -[/heap_bij_merge_shared[?[??]]?].
+      by simplify_option_eq.
+    + move => pii pi o /= ?.
+      rewrite lookup_union.
+      rewrite map_filter_lookup_true. 2: { move => *. rewrite elem_of_hb_shared_s. naive_solver. }
+      destruct (decide (pi ∈ hb_shared_i bijb')) as [Hpi'|Hpi'].
+      all: rewrite elem_of_hb_shared_i in Hpi'; destruct_all?.
+      * rewrite map_filter_lookup_None_2.
+        2: { right. move => *. rewrite !elem_of_hb_shared_s elem_of_hb_shared_i /=. naive_solver. }
+        rewrite right_id_L.
+        rewrite heap_through_bij_is_Some' //.
+        split. { apply Hh. rewrite heap_bij_merge_shared. naive_solver. }
+        move => ???/heap_through_bij_Some[ps'[?[?[??]]]]. simplify_bij.
+        move: (Hh pii ps' o) => [|_ Hv]. { rewrite heap_bij_merge_shared. naive_solver. }
+        efeed pose proof Hv as Hv'; [done..|].
+        move: Hv'. rewrite val_in_bij_merge => -[?[Hv1 Hv2]].
+        unfold val_in_bij in Hv1, Hv2. repeat case_match => //; destruct_all?; simplify_option_eq => //.
+        split; [done|]. congruence.
+      * destruct (h_heap (heap_through_bij bijb' h') !! (pi, o)) as [|] eqn: Hht => /=.
+        { move: Hht => /heap_through_bij_Some. naive_solver. }
+        rewrite left_id.
+        rewrite map_filter_lookup_true. 2: { move => *. rewrite elem_of_hb_shared_i. naive_solver. }
+        move: (Hpi pii o) => <-. 2: {
+          rewrite heap_bij_merge_player_i. right. split!; [done|]. by rewrite elem_of_hb_shared_i.
+        }
+        revert select (heap_in_bij bija hi hib) => Hhbij.
+        move: (Hhbij pii pi o) => [|HS Hv]. { naive_solver. }
+        rewrite HS. split; [done|]. move => ????. apply: val_in_bij_mono; [naive_solver|].
+        unfold heap_bij_extend in *. naive_solver.
+    + move => pi o /=. rewrite elem_of_hb_player_s => ?. rewrite lookup_union_r.
+      2: { apply map_filter_lookup_None. right. move => ??. rewrite elem_of_hb_shared_s. naive_solver. }
+      rewrite map_filter_lookup_true //.
+      move => ??. rewrite elem_of_hb_shared_s. naive_solver.
+    + apply: heap_preserved_mono; [done|]. move => ?.
+      rewrite {1}elem_of_hb_player_i /= heap_bij_merge_player_i. naive_solver.
+    + etrans; [|done]. by rewrite heap_bij_merge_dom.
+    + rewrite vals_of_event_event_set_vals_heap. 2: rewrite fmap_length; solve_length.
+      rewrite Forall2_fmap_l. apply Forall_Forall2_diag, Forall_forall => ?/= /elem_of_list_lookup [? Hin].
+      apply val_through_in_bij => ??. simplify_eq.
+      move: Hvs => /(Forall2_lookup_r _ _ _ _ _)/(_ Hin)[v [?]]. destruct v => //=.
+      rewrite heap_bij_merge_shared. naive_solver.
+    + move => pi ps o /= ?.
+      destruct (decide (pi ∈ hb_shared_s bija')) as [Hpi'|Hpi'];
+        rewrite elem_of_hb_shared_s in Hpi'; destruct_all?.
+      * rewrite lookup_union.
+        rewrite map_filter_lookup_true. 2: { move => *. rewrite elem_of_hb_shared_s. naive_solver. }
+        rewrite map_filter_lookup_None_2.
+        2: { right. move => *. rewrite elem_of_hb_shared_s elem_of_hb_shared_i. naive_solver. }
+        rewrite right_id_L.
+        rewrite heap_through_bij_is_Some' //. split; [done|].
+        move => ??. rewrite heap_through_bij_Some => ? ?. destruct_all?; simplify_bij.
+        eapply val_through_in_bij => ??.
+        move: (Hh pi0 ps0 o) => [|]. { rewrite heap_bij_merge_shared. naive_solver. }
+        simplify_option_eq. revert select (h_heap h' !! _ = Some _) => ->. move => [_ [//|v' ?]] Hv.
+        efeed pose proof Hv as Hv'; [done..|]. destruct v' => //; simplify_eq/=.
+        move: Hv'. rewrite heap_bij_merge_shared. naive_solver.
+      * rewrite lookup_union.
+        rewrite map_filter_lookup_None_2. 2: { right. move => *. rewrite elem_of_hb_shared_s. naive_solver. }
+        rewrite map_filter_lookup_true. 2: { move => *. rewrite elem_of_hb_shared_s. naive_solver. }
+        rewrite left_id_L.
+        move: (Hps ps o) => <-. 2: {
+          rewrite heap_bij_merge_player_s. right. eexists _. split; [done|]. apply default_eq_Some'.
+          move => [|[]]; [naive_solver|naive_solver|]. move => ?.
+          move: Hbij1e =>/set_eq/(_ pi). rewrite elem_of_hb_player_s. set_solver.
+        }
+        revert select (heap_in_bij bijb hib hs) => Hhbij.
+        move: (Hhbij pi ps o) => [|HS Hv]. { naive_solver. }
+        rewrite HS. split; [done|]. move => ????. apply: val_in_bij_mono; [naive_solver|].
+        unfold heap_bij_extend in *. naive_solver.
+    + apply: heap_preserved_mono; [done|].
+      move => ?. rewrite heap_bij_merge_player_s elem_of_hb_player_s. naive_solver.
+    + move => pi o /=. rewrite elem_of_hb_player_i => ?. rewrite lookup_union_r.
+      2: { apply map_filter_lookup_None. right. move => /=?/heap_through_bij_Some[?[?[/hb_disj??]]]. naive_solver. }
+      rewrite map_filter_lookup_true //.
+      move => ??. rewrite elem_of_hb_shared_i /=. right => -[? /hb_disj]. naive_solver.
+  - move => bijb' vsb hb' [Hextendb [Henvb_s Henvb_i]] Hdhb Hpsb Hvsb Hhb Hpb_i Hpb_s ??.
+    move => bija' vsa ha' [Hextenda [Henva_s Henva_i]] Hdha Hpsa Hvsa Hha Hpa_i Hpa_s ??.
+    destruct_all?; simplify_eq/=.
+    rewrite ->heap_of_event_event_set_vals_heap in *.
+    rewrite ->vals_of_event_event_set_vals_heap in *. 2: solve_length.
+    split!.
+    + split => /=.
+      * move => ??. rewrite !heap_bij_merge_shared. bij_solver.
+      * split; apply set_eq => ?.
+        -- rewrite !heap_bij_merge_player_s. f_equiv.
+           ++ rewrite -!elem_of_hb_player_s. by rewrite Henvb_s.
+           ++ setoid_rewrite default_eq_neq => //. setoid_rewrite <-elem_of_hb_player_s.
+              f_equiv => ?. rewrite -Henva_s. revert select (hb_player_s Env bija = ∅) => ->. set_solver.
+        -- rewrite !heap_bij_merge_player_i. f_equiv.
+           ++ rewrite -!elem_of_hb_player_i. set_solver.
+           ++ naive_solver.
+    + etrans; [|done]. by rewrite heap_bij_merge_dom.
+    + etrans; [|done]. move => ?. by rewrite heap_bij_merge_provs_i.
+    + elim: Hvsa (vals_of_event e.2) Hvsb. { move => *. decompose_Forall_hyps. econs. }
+      move => va vab {}vsa {}vsb ?? IH ??. decompose_Forall_hyps. econs; [|naive_solver].
+      apply val_in_bij_merge. naive_solver.
+    + by apply: heap_in_bij_merge.
+    + apply: heap_preserved_mono; [done|].
+      move => ?. rewrite heap_bij_merge_player_i elem_of_hb_player_i. naive_solver.
+    + apply: heap_preserved_mono; [done|].
+      move => ?. rewrite heap_bij_merge_player_s elem_of_hb_player_s.
+      setoid_rewrite default_eq_neq => //. setoid_rewrite <-elem_of_hb_player_s. set_solver.
+    + instantiate (1:=True%I). iIntros "? !>". done.
+    + by rewrite -Henva_s.
+Qed.
+(*
 
 Local Ltac split_solve :=
   match goal with
-  | |- heap_in_bij ?p _ _ => is_evar p; eassumption
+  (* | |- heap_in_bij ?p _ _ => is_evar p; eassumption *)
+  | |- heap_in_bij _ _ _ => apply: heap_in_bij_mono; [eassumption|..]
   | |- event_set_vals_heap _ _ _ = event_set_vals_heap _ _ _ => reflexivity
   | |- heap_bij_extend ?p ?a ?b =>
       assert_fails (has_evar p); assert_fails (has_evar a); assert_fails (has_evar b); by etrans
-  | |- ?a ⊆ ?b =>
-      assert_fails (has_evar a); assert_fails (has_evar b); etrans; [eassumption|]
-  | |- ?a ⊆ ?b =>
-      assert_fails (has_evar a); assert_fails (has_evar b); etrans; [|eassumption]
+  (* | |- ?a ⊆ ?b => *)
+      (* assert_fails (has_evar a); assert_fails (has_evar b); etrans; [eassumption|] *)
+  (* | |- ?a ⊆ ?b => *)
+      (* assert_fails (has_evar a); assert_fails (has_evar b); etrans; [|eassumption] *)
+  | |- _ ⊆ heap_bij_map_player _ _ => apply heap_bij_map_player_subseteq_r
+  | |- heap_bij_map_player _ _ ⊆ _ => apply heap_bij_map_player_subseteq_l
   | |- heap_preserved ?p ?a ?b =>
       assert_fails (has_evar p); assert_fails (has_evar a); assert_fails (has_evar b); etrans; [eassumption|]
   end.
@@ -535,63 +1425,52 @@ Proof.
       (λ ips '(ImpHeapBij bij1 hi1) '(ImpHeapBij bij2 hi2) '(ImpHeapBij bij hi) _ _ ics1 ics2,
         ∃ bijm,
           ics1 = ics2 ∧
-          hb_bij bij1 ⊆ bijm ∧
-          hb_bij bij2 ⊆ bijm ∧
-          hb_bij bij ⊆ bijm ∧
-       ((ips = SPNone ∧ bijm = hb_bij bij ∧
-          hb_env bij1 ⊆ hb_env bij ∪ hb_prog bij2 ∧
-          hb_env bij2 ⊆ hb_env bij ∪ hb_prog bij1 ∧
-          hb_prog bij = hb_prog bij1 ∪ hb_prog bij2 ∧
-          hb_prog bij1 ## hb_prog bij2 ∧
-          heap_preserved (hb_prog bij1) hi1 hi ∧
-          heap_preserved (hb_prog bij2) hi2 hi) ∨
-        ((ips = SPLeft ∧ bijm = hb_bij bij1 ∧
-          hb_env bij1 = hb_env bij ∪ hb_prog bij2 ∧
-          hb_env bij2 ⊆ hb_env bij ∪ hb_prog bij1 ∧
-          hb_prog bij ⊆ hb_prog bij1 ∪ hb_prog bij2 ∧
-          hb_prog bij2 ## hb_env bij ∧
-          heap_preserved (hb_env bij) hi hi1 ∧
-          heap_preserved (hb_prog bij2) hi2 hi1) ∨
-         (ips = SPRight ∧ bijm = hb_bij bij2 ∧
-          hb_env bij1 ⊆ hb_env bij ∪ hb_prog bij2 ∧
-          hb_env bij2 = hb_env bij ∪ hb_prog bij1 ∧
-          hb_prog bij ⊆ hb_prog bij1 ∪ hb_prog bij2 ∧
-          hb_prog bij1 ## hb_env bij ∧
-          heap_preserved (hb_env bij) hi hi2 ∧
-          heap_preserved (hb_prog bij1) hi1 hi2)))). }
+          bij1 ⊆ bijm ∧
+          bij2 ⊆ bijm ∧
+          bij ⊆ bijm ∧
+       ((ips = SPNone ∧ bijm = bij ∧
+          hb_player Prog bij = hb_player Prog bij1 ∪ hb_player Prog bij2 ∧
+          hb_player Prog bij1 ## hb_player Prog bij2 ∧
+          heap_preserved (hb_player Prog bij1) hi1 hi ∧
+          heap_preserved (hb_player Prog bij2) hi2 hi) ∨
+        ((ips = SPLeft ∧ bijm = bij1 ∧
+          hb_player Env bij1 = hb_player Env bij ∪ hb_player Prog bij2 ∧
+          hb_player Prog bij2 ## hb_player Env bij ∧
+          heap_preserved (hb_player Env bij) hi hi1 ∧
+          heap_preserved (hb_player Prog bij2) hi2 hi1) ∨
+         (ips = SPRight ∧ bijm = bij2 ∧
+          hb_player Env bij2 = hb_player Env bij ∪ hb_player Prog bij1 ∧
+          hb_player Prog bij1 ## hb_player Env bij ∧
+          heap_preserved (hb_player Env bij) hi hi2 ∧
+          heap_preserved (hb_player Prog bij1) hi1 hi2)))). }
   { move => ?? [] /=*; naive_solver. }
-  { by rewrite left_id. } { by apply satisfiable_pure. }
-  { split!. all: set_solver. }
+  { by rewrite left_id. } { by apply satisfiable_pure_1. }
+  { split!.  all: rewrite /hb_player; unlock; set_solver. }
   all: move => [bij1 hi1] [bij2 hi2] [bij hi] ? ? ics1 ics2.
-  - move => e ics' e' /= *. unfold heap_bij_extend in *; destruct_all?; simplify_eq/=.
-    unshelve split!. 1: econstructor. all: shelve_unifiable. all: split!. all: split!.
-    1: { set_unfold; naive_solver. }
+  - move => e ics' e' /= *. unfold heap_bij_extend in *. destruct_all?; simplify_eq/=.
+    eexists (heap_bij_map_player (λ p2 p, if decide (p2 ∈ hb_player Prog bij2) then Env else p) bij).
+    split!.
+    { set_unfold.
+    1: {
+1: econstructor. all: shelve_unifiable. all: split!. all: split!.
     1: { apply: heap_preserved_mono; [done|]. set_unfold; naive_solver. }
     1: by iIntros "$".
     1: by destruct e.
-    1: { set_unfold; naive_solver. }
-    1: { set_unfold; naive_solver. }
     1: { apply: disjoint_mono; [apply hb_disj_priv| |done]. set_unfold; naive_solver. }
     1: { apply: heap_preserved_mono; [done|]. set_unfold; naive_solver. }
   - move => e ics' e' /= *. unfold heap_bij_extend in *; destruct_all?; simplify_eq/=.
     unshelve split!. 1: econstructor. all: shelve_unifiable. all: split!. all: split!.
-    1: { set_unfold; naive_solver. }
     1: { apply: heap_preserved_mono; [done|]. set_unfold; naive_solver. }
     1: by iIntros "$".
     1: by destruct e.
-    1: { set_unfold; naive_solver. }
-    1: { set_unfold; naive_solver. }
     1: { apply: disjoint_mono; [apply hb_disj_priv| |done]. set_unfold; naive_solver. }
     1: { apply: heap_preserved_mono; [done|]. set_unfold; naive_solver. }
   - move => [? e] /= *. unfold heap_bij_extend in *; destruct_all?; simplify_eq/=.
     unshelve split!. 1: econstructor. all: shelve_unifiable.
     all: split!; rewrite ?heap_of_event_event_set_vals_heap; split!. all: split!.
-    1: { set_unfold; naive_solver. }
     1: { rewrite vals_of_event_event_set_vals_heap //. by apply: Forall2_length. }
     1: { apply: heap_preserved_mono; [done|]. set_unfold; naive_solver. }
     1: { iIntros "[? $]". iStopProof. etrans; [done|]. by iIntros ">[_ $]". }
-    1: { set_unfold; naive_solver. }
-    1: { set_unfold; naive_solver. }
     1: { apply: disjoint_mono; [apply hb_disj_priv|done|]. set_unfold; naive_solver. }
     1: { apply: heap_preserved_mono; [done|]. set_unfold; naive_solver. }
     1: by destruct e.
@@ -600,22 +1479,16 @@ Proof.
     unshelve split!. 1: econstructor. all: shelve_unifiable.
     all: split!; rewrite ?heap_of_event_event_set_vals_heap; split!. all: split!.
     1: by destruct e.
-    1: { set_unfold; naive_solver. }
     1: { apply: heap_preserved_mono; [done|]. set_unfold; naive_solver. }
     1: { etrans; [done|]. iIntros ">[? $]". iStopProof. etrans; [done|]. by iIntros ">[_ $]". }
-    1: { set_unfold; naive_solver. }
-    1: { set_unfold; naive_solver. }
     1: { apply: disjoint_mono; [apply hb_disj_priv|done|]. set_unfold; naive_solver. }
     1: { apply: heap_preserved_mono; [done|]. set_unfold; naive_solver. }
   - move => [? e] /= *. unfold heap_bij_extend in *; destruct_all?; simplify_eq/=.
     unshelve split!. 1: econstructor. all: shelve_unifiable.
     all: split!; rewrite ?heap_of_event_event_set_vals_heap; split!. all: split!.
-    1: { set_unfold; naive_solver. }
     1: { rewrite vals_of_event_event_set_vals_heap //. by apply: Forall2_length. }
     1: { apply: heap_preserved_mono; [done|]. set_unfold; naive_solver. }
     1: { iIntros "[$ ?]". iStopProof. etrans; [done|]. by iIntros ">[_ $]". }
-    1: { set_unfold; naive_solver. }
-    1: { set_unfold; naive_solver. }
     1: { apply: disjoint_mono; [apply hb_disj_priv|done|]. set_unfold; naive_solver. }
     1: { apply: heap_preserved_mono; [done|]. set_unfold; naive_solver. }
     1: by destruct e.
@@ -624,11 +1497,8 @@ Proof.
     unshelve split!. 1: econstructor. all: shelve_unifiable.
     all: split!; rewrite ?heap_of_event_event_set_vals_heap; split!. all: split!.
     1: by destruct e.
-    1: { set_unfold; naive_solver. }
     1: { apply: heap_preserved_mono; [done|]. set_unfold; naive_solver. }
     1: { etrans; [done|]. iIntros ">[$ ?]". iStopProof. etrans; [done|]. by iIntros ">[_ $]". }
-    1: { set_unfold; naive_solver. }
-    1: { set_unfold; naive_solver. }
     1: { symmetry. apply: disjoint_mono; [apply hb_disj_priv|done|]. set_unfold; naive_solver. }
     1: { apply: heap_preserved_mono; [done|]. set_unfold; naive_solver. }
     Unshelve.
@@ -928,7 +1798,6 @@ Proof.
   1, 2: by simplify_map_eq. 1,2: by econs.
   unshelve eexists (heap_bij_add_prog l.1 bij1 _), []. { apply Hf. }
   split!.
-  { unfold heap_bij_extend. split!. set_solver. }
   { apply heap_in_bij_update_r; [|set_solver]. apply heap_in_bij_alloc_r; [done|set_solver]. }
   { apply heap_preserved_update_r; [|set_solver]. apply heap_preserved_alloc_r; [set_solver|done]. }
   { instantiate (1:=True%I). iIntros "? !>". done. }
@@ -969,3 +1838,4 @@ Proof.
   apply bij_alloc_opt_refines.
 Qed.
 End imp_heap_bij_example.
+*)
